generic/Zeta.Record.fsti
@@ -4,53 +4,32 @@ open FStar.BitVector
 open Zeta.App
 open Zeta.BinTree
 open Zeta.Hash
-open Zeta.Key
+open Zeta.Merkle
+open Zeta.GenKey
 
-(* information about a desc stored in a merkle node *)
-type desc_hash = 
-  | Empty: desc_hash
-  | Desc: k:key -> h:hash_value -> b:bool -> desc_hash
+type value (aprm: app_params) =
+  | AppV: v: app_value_nullable aprm.adm -> value aprm
+  | IntV: v: Merkle.value -> value aprm
 
-(* merkle value: information about left and right descendants *)
-type merkle_value = 
-  | MkValue: l:desc_hash -> r:desc_hash -> merkle_value
-
-let desc_hash_dir (v:merkle_value) (d:bin_tree_dir) = 
-  match d with
-  | Left -> MkValue?.l v
-  | Right -> MkValue?.r v
-
-let merkle_record = merkle_key & merkle_value
-
-let mv_points_to_none (v: merkle_value) (d:bin_tree_dir): bool =
-  desc_hash_dir v d = Empty
-
-let mv_points_to_some (v:merkle_value) (d:bin_tree_dir): bool = 
-  Desc? (desc_hash_dir v d) 
-
-let mv_pointed_key (v:merkle_value) (d:bin_tree_dir{mv_points_to_some v d}): key = 
-  Desc?.k (desc_hash_dir v d)
-
-let mv_pointed_hash (v:merkle_value) (d:bin_tree_dir{mv_points_to_some v d}): hash_value = 
-  Desc?.h (desc_hash_dir v d)
-
-let mv_points_to (v:merkle_value) (d:bin_tree_dir) (k:key): bool = 
-  mv_points_to_some v d && mv_pointed_key v d = k
-
-let mv_evicted_to_blum (v:merkle_value) (d:bin_tree_dir {mv_points_to_some v d}): bool =
-  Desc?.b (desc_hash_dir v d)
+let compatible #aprm (k: key aprm) (v: value aprm) =
+  match k, v with
+  | AppK _, AppV _ -> true
+  | IntK _, IntV _ -> true
+  | AppK _, IntV _ -> false
+  | IntK _, AppV _ -> false
 
 (* a record is a union of merkle (internal) record and app record *)
-type record (aprm: app_params) =
-  | App: r: app_record aprm.adm -> record aprm
-  | Int: r: merkle_record -> record aprm
+let record (aprm: app_params) =
+  r:(key aprm & value aprm){ let k,v = r in compatible k v  }
 
-let value_t (#aprm: app_params) (r: record aprm): eqtype =
-  match r with
-  | App _ -> app_value_nullable aprm.adm
-  | Int _ -> merkle_value
+let value_t (#aprm: app_params) (k: key aprm) = v: value aprm {compatible k v}
 
-let update (#aprm: app_params) (r: record aprm) (v: value_t r) =
-  match r with
-  | App (k,_) -> App (k,v)
-  | Int (k,_) -> Int (k,v)
+let key_of (#aprm: app_params) (r: record aprm)
+  = let k, _ = r in k
+
+let value_of (#aprm: app_params) (r: record aprm)
+  = let _, v = r in v
+
+let to_merkle_value (#aprm: app_params) (v: value aprm { IntV? v })
+  = let IntV v = v in
+    v
