high2/Zeta.High.Verifier.fsti
@@ -3,35 +3,65 @@ module Zeta.High.Verifier
 open Zeta.App
 open Zeta.Time
 open Zeta.Thread
-open Zeta.Key
+open Zeta.GenKey
 open Zeta.Record
-
-(* union of internal (merkle) keys and app keys *)
-type key (app: app_params) =
-  | IntKey: k:merkle_key -> key app
-  | AppKey: k: app_key app.adm -> key app
-
-(* the record type once we fix a key *)
-let record_t #aprm (k: key aprm)
-  = match k with
-    | IntKey k -> r: record aprm { Int? r /\ (let Int (mk, _) = r in mk = k) }
-    | AppKey k -> r: record aprm { App? r /\ (let App (ak, _) = r in ak = k) }
+open Zeta.HashFunction
 
 (* for records in the store, how were they added? *)
 type add_method =
   | MAdd: add_method       (* AddM *)
   | BAdd: add_method         (* AddB *)
 
-(* verifier store entry *)
-type vstore_entry (#aprm: app_params) (k:key aprm) =
-  | VStore: r:record_t k -> am: add_method -> vstore_entry k
+(* verifier store entry indexed by a key k *)
+type vstore_entry (#aprm: app_params) (k:key aprm) = {
+  r:  r:record aprm {let kc,_ = r in kc = k};
+  am: add_method;
+}
 
 (* verifier store is a subset of (k,v) records *)
 (* we also track how the key was added merkle/blum *)
-let vstore (aprm: app_params) = (k:key aprm) -> option (vstore_entry k)
+let store_t (aprm: app_params) = (k:key aprm) -> option (vstore_entry k)
+
+(* does the store contain a key *)
+let store_contains (#aprm: app_params) (st:store_t aprm) (k:key aprm)
+  = Some? (st k)
+
+(* lookup the value of a key in the store *)
+let stored_value (#aprm: app_params) (st:store_t aprm) (k:key aprm{store_contains st k})
+  = let _, v = (Some?.v (st k)).r in
+    v
+
+(* add method of a key in the store *)
+let add_method_of (#aprm: app_params) (st:store_t aprm) (k:key aprm{store_contains st k})
+  = (Some?.v (st k)).am
+
+(* update the store *)
+let update_store (#aprm: app_params) (st:store_t aprm)
+                 (k:key aprm{store_contains st k})
+                 (v:value_t k):
+  Tot (st':store_t aprm {store_contains st' k /\ stored_value st' k = v})
+  = let am = add_method_of st k in
+    let r = k, v in
+    fun k' -> if k' = k then Some ( { r; am } ) else st k'
+
+(* add a new record to the store *)
+let add_to_store (#aprm: app_params)
+                 (st:store_t aprm)
+                 (k:key aprm)
+                 (v:value_t k)
+                 (am:add_method):
+  (st':store_t aprm {store_contains st' k /\ stored_value st' k = v})
+  = let r = k,v in
+    fun k' -> if k' = k then Some ({ r; am }) else st k'
+
+(* evict a key from a store *)
+let evict_from_store (#aprm: app_params)
+                     (st:store_t aprm)
+                     (k:key aprm{store_contains st k}) =
+  fun k' -> if k' = k then None else st k'
 
 (* per-thread state of the high-level verifier *)
-noeq type vtls (app: app_params) = {
+noeq type vtls_t (app: app_params) = {
   (* is the verifier valid *)
   valid: bool;
 
@@ -42,5 +72,51 @@ noeq type vtls (app: app_params) = {
   clock: timestamp;
 
   (* verifier store *)
-  st: vstore app;
+  st: store_t app;
 }
+
+val fail (#aprm: app_params) (vtls: vtls_t aprm): v:vtls_t aprm{v.valid = false}
+
+let addm (#aprm: app_params)
+         (r:record aprm)
+         (k: key)
+         (k':key)
+         (vs: vtls_t {vs.valid}): vtls_t aprm
+  = let st = vs.st in
+    let (kc,v) = r in
+    let open Zeta.GenKey in
+    let open Zeta.Merkle in
+    (* the key of the record should be identical to "slot" k *)
+    if k <> kc then fail vs
+    (* check k is a proper desc of k' *)
+    else if not (is_proper_desc k k') then fail vs
+    (* check store contains k' *)
+    else if not (store_contains st k') then fail vs
+    (* check store does not contain k *)
+    else if store_contains st k then fail vs
+    else
+      let v' = to_merkle_value (stored_value st k') in
+      let d = desc_dir k k' in
+      let dh' = desc_hash v' d in
+      let h = hashfn v in
+      match dh' with
+      | Empty -> if v = init_value k then
+                 let v'_upd = update_merkle_value v' d k h false in
+                 let st_upd = update_store st k' (MVal v'_upd) in
+                 let st_upd2 = add_to_store st_upd k v MAdd in
+                 update_thread_store vs st_upd2
+               else Failed
+    | Desc k2 h2 b2 -> if k2 = k then
+                         if h2 = h && b2 = false then
+                           update_thread_store vs (add_to_store st k v MAdd)
+                          else Failed
+                       else if v <> init_value k then Failed
+                       else if not (is_proper_desc k2 k) then Failed
+                       else
+                         let d2 = desc_dir k2 k in
+                         let mv = to_merkle_value v in
+                         let mv_upd = update_merkle_value mv d2 k2 h2 b2 in
+                         let v'_upd = update_merkle_value v' d k h false in
+                         let st_upd = update_store st k'(MVal  v'_upd) in
+                         let st_upd2 = add_to_store st_upd k (MVal mv_upd) MAdd in
+                         update_thread_store vs st_upd2
