generic/Zeta.GenKey.fsti
@@ -1,0 +1,29 @@
+module Zeta.GenKey
+
+open Zeta.App
+open Zeta.Key
+open Zeta.Merkle
+
+module BT = Zeta.BinTree
+
+type key (aprm: app_params) =
+  | AppK: k: app_key aprm.adm -> key aprm
+  | IntK: k: Merkle.key -> key aprm
+
+(* extend proper desc relationship to general keys *)
+let is_proper_desc #aprm (kd: key aprm) (ka: key aprm)
+  = match kd, ka with
+    | _, AppK _ -> false (* nothing is a proper descendant of an application key *)
+    | AppK kd, IntK ka ->
+      let kd: leaf_key = aprm.keyhashfn kd in
+      BT.is_proper_desc kd ka
+    | IntK kd, IntK ka ->
+      BT.is_proper_desc kd ka
+
+let desc_dir #aprm (kd: key aprm) (ka: key aprm { is_proper_desc kd ka })
+  = match kd, ka with
+    | AppK kd, IntK ka ->
+      let kd = aprm.keyhashfn kd in
+      BT.desc_dir kd ka
+    | IntK kd, IntK ka ->
+      BT.desc_dir kd ka
