generic/Zeta.HashFunction.fsti
@@ -1,0 +1,7 @@
+module Zeta.HashFunction
+
+open Zeta.Hash
+open Zeta.App
+open Zeta.Record
+
+val hashfn (#aprm: app_params) (v: value aprm): Tot hash_value
