generic/Zeta.Merkle.fsti
@@ -1,0 +1,42 @@
+module Zeta.Merkle
+
+open Zeta.BinTree
+open Zeta.Hash
+open Zeta.Key
+
+(* a merkle key *)
+let key = merkle_key
+
+(* information about a desc stored in a merkle node *)
+type desc_hash_t =
+  | Empty: desc_hash_t
+  | Desc: k:key -> h:hash_value -> b:bool -> desc_hash_t
+
+(* merkle value: information about left and right descendants *)
+type value = {
+  left: desc_hash_t;
+  right: desc_hash_t;
+}
+
+let desc_hash (v:value) (d:bin_tree_dir) =
+  match d with
+  | Left -> v.left
+  | Right -> v.right
+
+let points_to_none (d:bin_tree_dir) (v: value) : bool =
+  desc_hash v d = Empty
+
+let points_to_some (v:value) (d:bin_tree_dir): bool =
+  Desc? (desc_hash v d)
+
+let pointed_key (v:value) (d:bin_tree_dir{points_to_some v d}): key =
+  Desc?.k (desc_hash v d)
+
+let pointed_hash (v:value) (d:bin_tree_dir{points_to_some v d}): hash_value =
+  Desc?.h (desc_hash v d)
+
+let points_to (v:value) (d:bin_tree_dir) (k:key): bool =
+  points_to_some v d && pointed_key v d = k
+
+let evicted_to_blum (v:value) (d:bin_tree_dir {points_to_some v d}): bool =
+  Desc?.b (desc_hash v d)
